Verify trie building

src/Utils/EGraph/Semantics.v
@@ -217,6 +217,7 @@ Section WithMap.
   
   Context (symbol_map : forall A, map.map symbol A)
     (symbol_map_plus : map_plus symbol_map)
+    (symbol_map_plus_ok : @map_plus_ok _ _ symbol_map_plus)
     (symbol_map_ok : forall A, map.ok (symbol_map A)).
 
   Context 
@@ -2315,7 +2316,9 @@ Abort.
 
   
   (*TODO: move to coqutil *)
-  Lemma extends_put_None A (i : idx_map A) k v
+  Lemma extends_put_None {key value : Type} {map : map.map key value} `{@map.ok _ _ map}
+                         `{Eqb_ok key}
+    (i : map) k v
     : map.get i k = None -> map.extends (map.put i k v) i.
   Proof.
     repeat intro.
@@ -3260,9 +3263,7 @@ Abort.
     open_ssm; destruct e; break; try eexists; intros; cbn; eauto.
   Qed.
 
- (*
-  Record rule_sound_for_evaluation (*m*) i r : Prop :=.
-  *)
+ 
 
   Definition atom_of_access f (access : list nat * nat) args : atom :=
     Build_atom f (map (fun n => nth n args default) (fst access))
@@ -3274,39 +3275,27 @@ Abort.
   
   Arguments query_ptr_symbol {idx symbol}%type_scope e.
   Arguments query_ptr_ptr {idx symbol}%type_scope e.
+  
+  Definition lookup_trie_sound_for_model i tries
+    (query_clauses : symbol_map (idx_map (list nat * nat)%type)) f x :=
+    forall qc' access,
+      map.get query_clauses f = Some qc' ->
+      map.get qc' x = Some access ->
+      forall tries',
+        map.get tries f = Some tries' ->
+        forall t1 t2,
+          map.get tries' x = Some (t1, t2) ->
+          trie_sound_for_model i f t1 access
+          /\ trie_sound_for_model i f t2 access.
 
   Definition ptr_trie_sound_for_model i tries
     (query_clauses : symbol_map (idx_map (list nat * nat)%type))
     (p : erule_query_ptr _ _) :=
-    match map.get tries p.(query_ptr_symbol),
-       map.get query_clauses p.(query_ptr_symbol) with
-    | Some tries', Some qc' =>
-        match map.get tries' p.(query_ptr_ptr),
-          map.get qc' p.(query_ptr_ptr) with
-        | Some (t1, t2), Some access =>
-            trie_sound_for_model i p.(query_ptr_symbol) t1 access
-            /\ trie_sound_for_model i p.(query_ptr_symbol) t2 access
-        | _, _ => False
-        end
-    | _, _ => False
-    end.
+    lookup_trie_sound_for_model i tries query_clauses p.(query_ptr_symbol) p.(query_ptr_ptr).
 
   Definition tries_sound_for_model i tries
     (query_clauses : symbol_map (idx_map (list nat * nat)%type)) :=
-    forall f x qc' access,
-      map.get query_clauses f = Some qc' ->
-      map.get qc' x = Some access ->
-      match map.get tries f with
-      | Some tries' =>
-          match map.get tries' x with
-          | Some (t1, t2) =>
-              trie_sound_for_model i f t1 access
-              /\ trie_sound_for_model i f t2 access
-          | None => False
-          end
-      | None => False
-      end.
-
+    forall f x, lookup_trie_sound_for_model i tries query_clauses f x.
   
   Arguments query_vars {idx symbol}%type_scope _.
   Arguments write_vars {idx symbol}%type_scope _.
@@ -3350,7 +3339,7 @@ Abort.
   Arguments write_clauses {idx symbol}%type_scope _.
   Arguments write_unifications {idx symbol}%type_scope _.
       
-  Record rule_sound_for_evaluation i qc (r : erule idx symbol) : Prop :=
+  Record rule_sound_for_evaluation' i qc (r : erule idx symbol) : Prop :=
     {
       (* rule wfness properties *)
       vars_NoDup : NoDup (r.(write_vars)++r.(query_vars));
@@ -3509,8 +3498,8 @@ Abort.
       basic_utils_crush.
   Qed.
 
-  Lemma exec_write_sound i r assign_vals qc
-    : rule_sound_for_evaluation i qc r ->
+  Lemma exec_write_sound' i r assign_vals qc
+    : rule_sound_for_evaluation' i qc r ->
       Datatypes.length r.(query_vars) = Datatypes.length assign_vals ->
       query_assignment_sound i qc (combine r.(query_vars) assign_vals) r.(query_clause_ptrs) ->
       state_sound_for_model m i
@@ -3788,16 +3777,72 @@ Abort.
     repeat (eapply eq_sound_monotone; [eassumption| eauto]).
   Qed.
 
+   Record wf_erule (r : erule idx symbol) : Prop :=
+    {
+      wf_vars_NoDup : NoDup (r.(write_vars)++r.(query_vars));
+      wf_write_clauses_well_scoped
+      : incl (flat_map (fun a => atom_ret a :: atom_args a)
+                r.(write_clauses)) (r.(query_vars) ++ r.(write_vars));
+      wf_write_unifications_well_scoped
+      : incl (flat_map (fun p => [fst p; snd p])
+                r.(write_unifications)) (r.(query_vars) ++ r.(write_vars));
+      wf_rule_vars_covered : incl r.(query_vars)
+                                   (flat_map query_ptr_args
+                                      (as_list r.(query_clause_ptrs)));
+      }.
+      
+   Record rule_sound_for_assignment i qc (r : erule idx symbol)
+     (rule_assignment : named_list idx (named_list idx idx -> idx)): Prop :=
+    {
+      assign_rule_assignment_dom
+      : r.(write_vars) = (map fst rule_assignment);
+      assign_rule_assignment_sound
+      : forall x f, In (x,f) rule_assignment ->
+                    forall qa, query_assignment_sound i qc qa r.(query_clause_ptrs) ->
+                               eq_sound_for_model m i (f qa) (f qa);
+      assign_write_assignment :=
+        fun qa => (named_map (fun f => f qa) rule_assignment) ++ qa;
+      assign_clauses_sound
+      : forall qa, query_assignment_sound i qc qa r.(query_clause_ptrs) ->
+                   all (fun c => atom_sound_for_model m i (atom_subst (assign_write_assignment qa) c))
+                     r.(write_clauses);
+      assign_eqns_sound
+      : forall qa, query_assignment_sound i qc qa r.(query_clause_ptrs) ->
+                   all (fun '(x,y) =>
+                          exists vx vy,
+                            In (x,vx) qa
+                            /\ In (y,vy) qa
+                            /\ eq_sound_for_model m i vx vy)
+                     r.(write_unifications);
+    }.
+
+   Definition rule_sound_for_evaluation i qc r : Prop :=
+     wf_erule r /\ forall i', map.extends i' i -> exists a, rule_sound_for_assignment i' qc r a.
+
+  
+  Lemma exec_write_sound i r assign_vals qc
+    : rule_sound_for_evaluation i qc r ->
+      Datatypes.length r.(query_vars) = Datatypes.length assign_vals ->
+      query_assignment_sound i qc (combine r.(query_vars) assign_vals) r.(query_clause_ptrs) ->
+      state_sound_for_model m i
+        (exec_write idx Eqb_idx idx_succ idx_zero symbol symbol_map idx_map
+           idx_trie analysis_result r assign_vals)
+        (fun (_ : idx_map (domain m)) (_ : unit) => True).
+  Proof.
+    intros; eapply exec_write_sound'; eauto.
+    edestruct H1 as [ [] [? [] ] ]; eauto with utils.
+    econstructor; eauto.
+  Qed.
+
   Lemma monotone_rule_sound_for_evaluation
     : monotone2 rule_sound_for_evaluation.
   Proof.
     repeat intro.
     destruct H2; econstructor; intros; eauto.
-    { eapply eq_sound_monotone; try eassumption.
-      eapply rule_assignment_sound; eauto.
-     (* fail (*TODO: issue! antitone*).
-      eapply eq_sound_monotone; try eassumption.*)
-  Abort. 
+    eapply map_extends_trans in H1; try eassumption.
+    eapply H3 in H1; break.
+    exists x; eauto.
+  Qed.
     
   Lemma process_erule'_sound i tries frontier_idx (r : erule _ _) qc
     : tries_sound_for_model i tries qc ->
@@ -3813,24 +3858,38 @@ Abort.
     apply state_sound_for_model_Miter with (P:= fun _ _ => True);
       intros; auto.
     eapply exec_write_sound; eauto.
-    (*
-    TODO: need var coverage for assignment length lemma
-    TODO: monotone rule_sound_for_evaluation.
-    TODO:  where to get query_assignment_sound?
-     *)
-    Abort.
+    1: eapply monotone_rule_sound_for_evaluation; now eauto.
+    {
+      unfold intersection_keys in *.
+      admit (*TODO: parameterized on spaced_list_intersect*).
+    }
+    {
+      (*TODO: prove from tries_sound_for_model*)
+      
+      admit (*TODO: parameterized on spaced_list_intersect*).
+    }
+  Admitted.
+
+  Lemma tries_sound_for_model_monotone
+    : monotone2 tries_sound_for_model.
+  Admitted.
   
-  (*TODO assumptions on tries*)
-  Lemma process_erule_sound i tries r qc (*TODO: relate qc and r*)
+  Lemma process_erule_sound i tries r qc
     :  tries_sound_for_model i tries qc ->
+       rule_sound_for_evaluation i qc r ->
        state_sound_for_model m i
         (process_erule idx Eqb_idx idx_succ idx_zero symbol symbol_map
            idx_map idx_trie analysis_result spaced_list_intersect tries r)
         (fun _ _ => True).
   Proof.
     intros.
-    
-  Abort.
+    unfold process_erule.
+    apply state_sound_for_model_Miter with (P:= fun _ _ => True);
+      intros; auto.
+    eapply process_erule'_sound; eauto.
+    { eapply tries_sound_for_model_monotone; eauto. }
+    { eapply monotone_rule_sound_for_evaluation; eauto. }
+  Qed.
 
   (*
     Definition ptr_trie_sound_for_model i tries (p : erule_query_ptr) :=
@@ -3849,16 +3908,321 @@ Abort.
 query_clauses symbol_map (idx_map (list nat * nat))
 *)
 
-  Lemma run1_iter_sound i rs rb_fuel
+  (*TODO: move to defining file*)
+  Arguments query_clauses {idx symbol}%type_scope {symbol_map idx_map}%function_scope r.
+
+  Context (idx_map_plus_ok : @map_plus_ok _ _ idx_map_plus).
+
+  Lemma empty_trie_sound_for_model i f p
+    : trie_sound_for_model i f map.empty p.
+  Proof.
+    repeat intro;
+      basic_utils_crush.
+  Qed.
+  Hint Resolve empty_trie_sound_for_model : utils.
+  
+  Lemma trie_sound_for_model_put i f r1 access l0
+    : trie_sound_for_model i f r1 access ->
+      atom_sound_for_model m i (atom_of_access f access l0) ->
+      trie_sound_for_model i f (map.put r1 l0 tt) access.
+  Proof.
+    unfold trie_sound_for_model.
+    intros.
+    eqb_case k l0; eauto.
+    rewrite map.get_put_diff in * by auto.
+    eauto.
+  Qed.
+
+  
+  Lemma insert_nth acc n v l1 d
+    : insert idx Eqb_idx acc n v = Some l1 ->
+      nth n l1 d = Some v.
+  Proof.
+    revert acc l1; induction n;
+      basic_goal_prep;
+      repeat case_match; inversions; try congruence;
+      cbn; eauto;
+      basic_utils_crush;
+      unfold option_map in H1; case_match; try congruence;
+      inversions;
+      cbn; eauto.
+  Qed.
+
+  Lemma match_clause'_ret l n k v l1 acc d
+    : match_clause' l n k v acc = Some l1 ->
+      nth n l1 d = Some v.
+  Proof.
+    revert k l1 acc.
+    induction l;
+      basic_goal_prep;
+      repeat case_match; try congruence; eauto using insert_nth.
+  Qed.
+
+  (*TODO: move to Base.v*)
+  Ltac inject f :=
+    lazymatch goal with
+      |- ?A = ?B =>
+        enough (f A = f B) by (cbn; congruence)
+    end.
+
+  Fixpoint match_list_leq (l1 l2 : list (option idx)) :=
+    match l1, l2 with
+    | [], _ => True
+    | None::l1', _::l2' => match_list_leq l1' l2'
+    | (Some x)::l1', (Some y)::l2' =>
+        x = y /\ match_list_leq l1' l2'
+    | _, _ => False
+    end.
+
+  Lemma match_list_leq_refl l : match_list_leq l l.
+  Proof.
+    induction l; basic_goal_prep; repeat case_match; basic_utils_crush.
+  Qed.
+  Hint Resolve match_list_leq_refl : utils.
+  
+  Lemma match_list_leq_trans : Transitive match_list_leq.
+  Proof.
+    intro l.
+    induction l; basic_goal_prep;
+      repeat (case_match; basic_goal_prep); basic_utils_crush.
+  Qed.
+
+  Add Parametric Relation : (list (option idx)) match_list_leq
+    reflexivity proved by match_list_leq_refl
+    transitivity proved by match_list_leq_trans
+    as match_list_leq_rel.
+  
+  Lemma insert_monotone acc n v l'
+    : insert idx Eqb_idx acc n v = Some l' ->
+      match_list_leq acc l'.
+  Proof.
+    revert acc l'; induction n;
+      basic_goal_prep; auto; inversions.
+    {
+      case_match; cbn; intuition auto with utils.
+      case_match; inversions; cbn; intuition auto with utils.
+      eqb_case v i; inversions; cbn; intuition auto with utils.
+    }
+    case_match; cbn; intuition auto with utils.
+    case_match; cbn; intuition auto with utils.
+    all: destruct (insert idx Eqb_idx acc n v) eqn:Hins;
+      cbn in *; inversions; eauto; try tauto.
+  Qed.
+
+  Lemma match_clause'_monotone l n k v l' acc
+    : match_clause' l n k v acc = Some l' ->
+      match_list_leq acc l'.
+  Proof.
+    revert k l' acc;
+    induction l;
+      basic_goal_prep;
+      repeat case_match; try congruence; cbn; eauto using insert_monotone.
+    etransitivity; eauto using insert_monotone.
+  Qed.
+
+  Lemma match_list_leq_nth l1 l2 x n0
+    : match_list_leq l1 l2 ->
+      nth n0 l1 default = Some x ->
+      nth n0 l2 default = Some x.
+  Proof.
+    unfold default, option_default.
+    revert l1 l2;
+      induction n0;
+      destruct l1, l2;
+      basic_goal_prep; subst; try tauto;
+      try congruence.
+    all: case_match; intuition subst; eauto.
+    case_match; intuition subst; eauto.
+  Qed.
+
+  (*TODO: not true?, needs more conditions. specifically, acc*)
+  Lemma match_clause'_args' l n k v l' acc
+    : match_clause' l n k v acc = Some l' ->
+      map (fun n0 : nat => nth n0 l' default) l = map Some k.
+  Proof.
+    revert k l' acc.
+    induction l;
+      basic_goal_prep;
+      repeat case_match; try congruence; cbn; auto.
+    f_equal; eauto.
+    eapply match_list_leq_nth; eauto using match_clause'_monotone.
+    eapply insert_nth; eauto.
+  Qed.
+  
+  Lemma match_clause'_args l n k v acc l0
+    : match_clause' l n k v acc = Some (map Some l0) ->
+      map (fun n0 : nat => nth n0 l0 default) l = k.
+  Proof.
+    intros.
+    apply match_clause'_args' in H1.
+    revert k H1.
+    induction l;
+      destruct k;
+      basic_goal_prep;
+      basic_utils_crush.
+    revert H2.
+    clear.
+    revert l0; induction a; destruct l0;
+      basic_goal_prep;
+      basic_utils_crush.
+  Qed.
+    
+  Lemma match_clause_atom_of_access f access k entry_value l0
+    : match_clause access k entry_value = Some l0 ->
+      atom_of_access f access l0 = Build_atom f k entry_value.
+  Proof.
+    unfold match_clause; break.
+    unfold atom_sound_for_model; cbn.
+    case_match; try congruence; intros.
+    unfold atom_of_access.
+    apply option_all_map_Some in H1; subst.
+    cbn.
+    f_equal.
+    2:{
+      inject (@Some idx).
+      rewrite <- map_nth.
+      eapply match_clause'_ret; eauto.
+    }      
+    { eapply match_clause'_args; eauto. }
+  Qed.
+
+  (*TODO: move to coqutil *)
+  Section MapFacts.
+    Context (key value : Type) (map : map.map key value) `{@map.ok _ _ map}.
+    
+    Lemma map_extends_empty  (m0 : map)
+      : map.extends map.empty m0 <-> m0 = map.empty.
+    Proof.
+      split; intros; subst; eauto with utils.
+      apply map.map_ext.
+      intros.
+      basic_utils_crush; eauto.
+      destruct (map.get m0 k) eqn:Hget; auto.
+      exfalso.
+      apply H2 in Hget.
+      basic_utils_crush.
+    Qed.
+    Hint Rewrite map_extends_empty : utils.
+
+    
+    Lemma map_extends_put_wkn (m0 m1 : map) k v
+      : map.get m1 k = None ->
+        map.extends m0 (map.put m1 k v) ->
+        map.extends m0 m1.
+    Proof.
+      repeat intro.
+      assert (x <> k) by congruence.
+      apply H3.
+      rewrite map.get_put_diff by auto.
+      auto.
+    Qed.
+
+    Lemma map_fold_spec_member' {R : Type} (P : map -> R -> Prop)
+      (f : R -> key -> value -> R) (r0 : R) (m0 : map)
+      : P map.empty r0 ->
+        (forall (k : key) (v : value) (m : map) (r : R),
+            map.get m0 k = Some v ->
+            map.get m k = None -> P m r -> P (map.put m k v) (f r k v)) ->
+        forall m, map.extends m0 m -> P m (map.fold f r0 m).
+    Proof.
+      intros ? ? m1.
+      pattern (map.fold f r0 m1).
+      revert m1.
+      apply map.fold_spec;
+        basic_goal_prep; basic_utils_crush.
+      eapply H3; eauto.
+      2:{
+        apply H5.
+        eapply map_extends_put_wkn; eauto.
+      }
+      {
+        apply H6; rewrite map.get_put_same; auto.
+      }
+    Qed.
+    
+    Lemma map_fold_spec_member {R : Type} (P : map -> R -> Prop)
+      (f : R -> key -> value -> R) (r0 : R) (m0 : map)
+      : P map.empty r0 ->
+        (forall (k : key) (v : value) (m : map) (r : R),
+            map.get m0 k = Some v ->
+            map.get m k = None -> P m r -> P (map.put m k v) (f r k v)) ->
+        P m0 (map.fold f r0 m0).
+    Proof.
+      intros;eapply map_fold_spec_member'; eauto with utils.
+    Qed.
+
+  End MapFacts.
+  Hint Rewrite map_extends_empty : utils.
+  
+  Lemma build_tries_for_symbol_sound i f qc' r0 x t1 t2 l n ep
+    : (forall k v, map.get r0 k = Some v ->
+                   atom_sound_for_model m i (Build_atom f k v.(entry_value _ _))) ->
+      map.get (build_tries_for_symbol idx Eqb_idx idx_map idx_map_plus idx_trie analysis_result 
+                 ep qc' r0) x = Some (t1, t2) ->
+      map.get qc' x = Some (l, n) ->
+      trie_sound_for_model i f t1 (l, n) /\ trie_sound_for_model i f t2 (l, n).
+  Proof.
+    intros Hsound Hget Hqc.
+    revert Hget.
+    unfold build_tries_for_symbol.
+    revert t1 t2.
+    apply map_fold_spec_member; eauto.
+    {
+      rewrite map_map_spec; eauto.
+      unfold option_map; case_match; try congruence; repeat inversions.
+      basic_goal_prep; subst; repeat inversions; intuition eauto with utils.
+    }
+    basic_goal_prep.
+    destruct v.
+    rewrite intersect_spec in *; eauto.
+    case_match; try congruence.
+    case_match; try congruence.
+    break.
+    inversions.
+    case_match.
+    2:{ apply H3; congruence. }
+    specialize (H3 _ _ eq_refl); break.
+    eqb_case entry_epoch ep; inversions; intuition eauto.
+    all: apply trie_sound_for_model_put; auto.
+    all: erewrite match_clause_atom_of_access; eauto.
+  Qed.
+  
+  Lemma build_tries_sound i rs
     : state_sound_for_model m i
+        (build_tries idx Eqb_idx symbol symbol_map symbol_map_plus idx_map idx_map_plus
+           idx_trie analysis_result rs)
+        (fun i' tries => tries_sound_for_model i' tries rs.(query_clauses)).
+  Proof.
+    open_ssm.
+    repeat intro.
+    rewrite intersect_spec in *; eauto.
+    repeat case_match; cbn; inversions; try tauto.
+    eapply build_tries_for_symbol_sound; eauto.
+    intros.
+    eapply atom_interpretation; eauto.
+    unfold atom_in_egraph, atom_in_db; cbn.
+    unfold db_map.
+    rewrite case_match_eqn0; cbn.
+    rewrite H1; cbn.
+    auto.
+  Qed.
+  
+  (*TODO: move*)
+  Arguments compiled_rules {idx symbol}%type_scope {symbol_map idx_map}%function_scope r.
+  
+  Lemma run1_iter_sound i rs rb_fuel
+    : all (rule_sound_for_evaluation i (query_clauses rs)) rs.(compiled_rules) ->
+      state_sound_for_model m i
         (Defs.run1iter idx Eqb_idx idx_succ idx_zero symbol Eqb_symbol
            symbol_map symbol_map_plus idx_map idx_map_plus idx_trie
            analysis_result spaced_list_intersect rs rb_fuel) 
         (fun _ _ => True).
   Proof.
     unfold Defs.run1iter.
+    intros.
     ssm_bind.
-    2:{
+    { apply build_tries_sound. }
+    {
       ssm_bind.
       1: apply increment_epoch_sound.
       ssm_bind.
@@ -3868,26 +4232,25 @@ query_clauses symbol_map (idx_map (list nat * nat))
       }
       apply state_sound_for_model_Miter with (P:= fun _ _ => True);
         intros; eauto.
-        admit.
+      eapply process_erule_sound; eauto.
+      { repeat (eapply tries_sound_for_model_monotone; try eassumption). }
+      {
+        eapply in_all in H1; eauto.
+        repeat (eapply monotone_rule_sound_for_evaluation; try eassumption).
+      }
     }
-    admit.
-  Admitted.
-    (*
-    Lemma build_tries_sound
-      : state_sound_for_model m i
-    (build_tries idx Eqb_idx symbol symbol_map symbol_map_plus idx_map
-       idx_map_plus idx_trie analysis_result rs) 
-    ?P*)
+  Qed.
     
   Lemma saturate_until'_sound i rb_fuel rs cond fuel P
-    : (forall i', map.extends i' i ->
+    : all (rule_sound_for_evaluation i (query_clauses rs)) rs.(compiled_rules) ->
+      (forall i', map.extends i' i ->
                   state_sound_for_model m i' cond (fun i2 (b:bool) => if b then P i2 else True)) ->
       monotone P ->
       forall i', map.extends i' i ->
       state_sound_for_model m i' (saturate_until' rs cond fuel rb_fuel)
         (fun i b => if b then P i else True).
   Proof.
-    intros Hcond HP.
+    intros Hrule Hcond HP.
     induction fuel;
       cbn [Defs.saturate_until'].
     { intros; eapply ret_sound_for_model'; auto. }
@@ -3897,7 +4260,12 @@ query_clauses symbol_map (idx_map (list nat * nat))
       destruct a.
       { eapply ret_sound_for_model'; auto. }
       eapply state_sound_for_model_Mseq.
-      { apply run1_iter_sound. }
+      {
+        apply run1_iter_sound.
+        eapply all_wkn; try eassumption.
+        intros.
+        repeat (eapply monotone_rule_sound_for_evaluation; try eassumption).
+      }
       {
         intros; eauto.
         eapply IHfuel.
@@ -3913,6 +4281,7 @@ query_clauses symbol_map (idx_map (list nat * nat))
     (* TODO: package rs properties together*)
     : all (const_rule_sound_for_evaluation i)
         (compiled_const_rules idx symbol symbol_map idx_map rs) ->
+      all (rule_sound_for_evaluation i (query_clauses rs)) rs.(compiled_rules) ->
       (forall i', map.extends i' i ->
                   state_sound_for_model m i' cond (fun i2 (b:bool) => if b then P i2 else True)) ->
       monotone P ->
@@ -3929,8 +4298,7 @@ query_clauses symbol_map (idx_map (list nat * nat))
     intros.
     eapply saturate_until'_sound; eauto.
     repeat (eapply map_extends_trans; try eassumption).
-  Qed.
-  
+  Qed.  
       
 End WithMap.
 
